Automata/LeadingZeros.lean
@@ -7,37 +7,57 @@ import Automata.Replicate
 import Automata.Pumping
 import Automata.Equality
 
-def padZeroes (m : ℕ) (x : List (Fin n → Fin (b+2))) : List (Fin n → Fin (b+2)) :=
+def padZeros (m : ℕ) (x : List (Fin n → Fin (b+2))) : List (Fin n → Fin (b+2)) :=
   List.replicate m (fun _ => 0) ++ x
 
-theorem padZeroes_add (a b : ℕ) (x : List (Fin n → Fin (k+2))) : padZeroes a (padZeroes b x) = padZeroes (a + b) x := by
-  simp only [padZeroes]
+theorem padZeros_add (a b : ℕ) (x : List (Fin n → Fin (k+2))) : padZeros a (padZeros b x) = padZeros (a + b) x := by
+  simp only [padZeros]
   rw[← List.append_assoc, List.replicate_append_add]
 
-theorem padZeroes_length (m : ℕ) (x : List (Fin n → Fin (b+2))) : (padZeroes m x).length = m + x.length := by
-  simp only [padZeroes]
+theorem padZeros_length (m : ℕ) (x : List (Fin n → Fin (b+2))) : (padZeros m x).length = m + x.length := by
+  simp only [padZeros]
   rw[List.replicate_append_length]
 
-theorem padZeroes_zero (m i: ℕ) (x : List (Fin n → Fin (b+2))) (h : i < m) : (padZeroes m x)[i]'(by simp only [padZeroes, List.length_append, List.length_replicate]; omega) = fun _ => 0 := by
-  simp only [padZeroes]
+theorem padZeros_zero (m i: ℕ) (x : List (Fin n → Fin (b+2))) (h : i < m) : (padZeros m x)[i]'(by simp only [padZeros, List.length_append, List.length_replicate]; omega) = fun _ => 0 := by
+  simp only [padZeros]
   rwa[List.getElem_of_replicate_append_left]
 
-theorem padZeroes_diff (a b: ℕ) (x y : List (Fin n → Fin (k+2))) (hab : a ≤ b) (h: (padZeroes a x) = (padZeroes b y)) : x = padZeroes (b - a) y := by
-  simp only [padZeroes] at *
+theorem padZeros_diff (a b: ℕ) (x y : List (Fin n → Fin (k+2))) (hab : a ≤ b) (h: (padZeros a x) = (padZeros b y)) : x = padZeros (b - a) y := by
+  simp only [padZeros] at *
   apply List.eq_diff_of_replicate_append_eq
   . exact h
   . exact hab
 
-def DFA.respectZero (dfa : DFA (Fin n → Fin (b+2)) state) : Prop := ∀ (x : List (Fin n → Fin (b+2))), ∀ m, dfa.eval x ↔ dfa.eval (padZeroes m x)
+def DFA.respectZero (dfa : DFA (Fin n → Fin (b+2)) state) : Prop := ∀ (x : List (Fin n → Fin (b+2))), ∀ m, dfa.eval x ↔ dfa.eval (padZeros m x)
 
-def NFA.respectZero [DecidableEq state] (nfa : NFA (Fin n → Fin (b+2)) state) : Prop := ∀ (x : List (Fin n → Fin (b+2))), ∀ m, nfa.eval x ↔ nfa.eval (padZeroes m x)
+def NFA.respectZero [DecidableEq state] (nfa : NFA (Fin n → Fin (b+2)) state) : Prop := ∀ (x : List (Fin n → Fin (b+2))), ∀ m, nfa.eval x ↔ nfa.eval (padZeros m x)
+
+theorem DFA.negate_respectZero (dfa : DFA (Fin n → Fin (b+2)) state) (h: dfa.respectZero) : dfa.negate.respectZero := by
+  rw[DFA.respectZero] at *
+  intro x m
+  specialize h x m
+  simp_all only [Bool.coe_iff_coe, negate_eval, Bool.not_eq_true']
+
+theorem DFA.union_respectZero (dfa1 : DFA (Fin n → Fin (b+2)) state1) (dfa2 : DFA (Fin n → Fin (b+2)) state2) (h1: dfa1.respectZero) (h2: dfa2.respectZero) : (dfa1.union dfa2).respectZero := by
+  rw[DFA.respectZero] at *
+  intro x m
+  specialize h1 x m
+  specialize h2 x m
+  simp_all only [Bool.coe_iff_coe, union_eval, Bool.or_eq_true]
+
+theorem DFA.intersection_respectZero (dfa1 : DFA (Fin n → Fin (b+2)) state1) (dfa2 : DFA (Fin n → Fin (b+2)) state2) (h1: dfa1.respectZero) (h2: dfa2.respectZero) : (dfa1.intersection dfa2).respectZero := by
+  rw[DFA.respectZero] at *
+  intro x m
+  specialize h1 x m
+  specialize h2 x m
+  simp_all only [Bool.coe_iff_coe, intersection_eval, Bool.and_eq_true]
 
 theorem equality_respectZero : (eqBase (b + 2) l m n).respectZero := by
   rw[DFA.respectZero]
   intro x c
   constructor
   intro h
-  rw[padZeroes]
+  rw[padZeros]
   rw[DFAO.eval, DFAO.evalFrom, DFAO.transFrom_of_append]
   nth_rw 1 [eqBase]
   simp only [Fin.isValue, beq_iff_eq]
@@ -56,7 +76,7 @@ theorem equality_respectZero : (eqBase (b + 2) l m n).respectZero := by
     simp_all only [List.mem_replicate, ne_eq, Fin.val_zero]
   . intro h
     contrapose h; simp_all only [Bool.not_eq_true]
-    rw[padZeroes]
+    rw[padZeros]
     rw[DFAO.eval, DFAO.evalFrom, DFAO.transFrom_of_append]
     nth_rw 1 [eqBase]
     simp only [Fin.isValue, beq_iff_eq]
@@ -71,9 +91,9 @@ theorem equality_respectZero : (eqBase (b + 2) l m n).respectZero := by
     apply eqBase_transFrom_zero 0 (List.replicate c fun _ ↦ 0) |>.mpr
     simp_all only [Fin.isValue, List.mem_replicate, ne_eq, Fin.val_zero, and_imp, implies_true, and_self]
 
-def DFA.acceptZero (dfa : DFA (Fin n → Fin (b+2)) state) : Prop := ∀ (x : List (Fin n → Fin (b+2))), (dfa.eval x → ∀ m, dfa.eval (padZeroes m x))
+def DFA.acceptZero (dfa : DFA (Fin n → Fin (b+2)) state) : Prop := ∀ (x : List (Fin n → Fin (b+2))), (dfa.eval x → ∀ m, dfa.eval (padZeros m x))
 
-def NFA.acceptZero [DecidableEq state] (nfa : NFA (Fin n → Fin (b+2)) state) : Prop := ∀ (x : List (Fin n → Fin (b+2))), (nfa.eval x → ∀ m, nfa.eval (padZeroes m x))
+def NFA.acceptZero [DecidableEq state] (nfa : NFA (Fin n → Fin (b+2)) state) : Prop := ∀ (x : List (Fin n → Fin (b+2))), (nfa.eval x → ∀ m, nfa.eval (padZeros m x))
 
 theorem DFA.acceptZero_of_respectZero (dfa : DFA (Fin n → Fin (b+2)) state) (h: dfa.respectZero) : dfa.acceptZero := by
   rw[DFA.acceptZero]
@@ -90,19 +110,19 @@ theorem NFA.acceptZero_of_respectZero [DecidableEq state] (nfa : NFA (Fin n → 
   exact h.mp hxo
 
 -- Bounded acceptance theorems: If a DFA/NFA accepts some representation of a input, then there is a bound on the number of leading zeros needed for acceptance
-theorem DFAO.bounded_out [Fintype state] (dfao : DFAO (Fin n → Fin (b+2)) state out) (x : List (Fin n → Fin (b+2))) (o: out)(h: ∀ (x : List (Fin n → Fin (b+2))), dfao.eval x = o → (∀ m, dfao.eval (padZeroes m x) = o)) : ∀ k, dfao.eval (padZeroes k x) = o → dfao.eval (padZeroes (Fintype.card state) x) = o := by
+theorem DFAO.bounded_out [Fintype state] (dfao : DFAO (Fin n → Fin (b+2)) state out) (x : List (Fin n → Fin (b+2))) (o: out)(h: ∀ (x : List (Fin n → Fin (b+2))), dfao.eval x = o → (∀ m, dfao.eval (padZeros m x) = o)) : ∀ k, dfao.eval (padZeros k x) = o → dfao.eval (padZeros (Fintype.card state) x) = o := by
   rintro k hkxo
   by_cases hkstate : k ≤ Fintype.card state
   . have: Fintype.card state = (Fintype.card state - k) + k := by omega
-    rw[this, ← padZeroes_add (Fintype.card state - k) k x]
+    rw[this, ← padZeros_add (Fintype.card state - k) k x]
     apply h
     exact hkxo
 
   simp only [not_le] at hkstate
   -- Question: How to get this kind of descent argument work in lean?
   . induction' hk : k - Fintype.card state using Nat.strong_induction_on  with d ih generalizing k
-    have hkxlen : Fintype.card state ≤ (padZeroes k x).length := by
-      simp only [padZeroes_length]
+    have hkxlen : Fintype.card state ≤ (padZeros k x).length := by
+      simp only [padZeros_length]
       omega
 
     obtain ⟨a, b', c, hkxabc, hablen, hne, hy⟩ := dfao.pumping_lemma_eval hkxo hkxlen
@@ -117,10 +137,10 @@ theorem DFAO.bounded_out [Fintype state] (dfao : DFAO (Fin n → Fin (b+2)) stat
     have habzero : ∀ i, ∀ (hi: i < a.length + b'.length),  (a ++ b')[i]' (by rw[List.length_append]; exact hi) = fun _ => 0 := by
       intro i hi
       rw[← List.getElem_append_left (a++b') c]
-      trans (padZeroes k x)[i]
+      trans (padZeros k x)[i]
       congr 1
       . exact hkxabc.symm
-      . apply padZeroes_zero k
+      . apply padZeros_zero k
         omega
       simp only [List.append_assoc, List.length_append]
       . omega
@@ -156,20 +176,20 @@ theorem DFAO.bounded_out [Fintype state] (dfao : DFAO (Fin n → Fin (b+2)) stat
     have hk : (List.replicate k (fun _ => 0)) = (List.replicate (a.length + b'.length) (fun _ => 0)) ++ (List.replicate (k - a.length - b'.length) (fun _ : Fin n => (0 : Fin (b + 2)))) := by
       simp[List.append_replicate_replicate]
       omega
-    have hcx : c = padZeroes (k - a.length - b'.length) x := by
+    have hcx : c = padZeros (k - a.length - b'.length) x := by
       rw[har, hbr] at hkxabc
-      rw[List.append_assoc, ← padZeroes, ← padZeroes, padZeroes_add] at hkxabc
-      simp only [padZeroes] at hkxabc
-      have : c = padZeroes (k - (a.length + b'.length)) x := by
+      rw[List.append_assoc, ← padZeros, ← padZeros, padZeros_add] at hkxabc
+      simp only [padZeros] at hkxabc
+      have : c = padZeros (k - (a.length + b'.length)) x := by
         apply List.eq_diff_of_replicate_append_eq
         . exact hkxabc.symm
         . omega
       rw[this]
       convert rfl using 2
       omega
-    have hac : a ++ c = padZeroes (k - b'.length) x := by
+    have hac : a ++ c = padZeros (k - b'.length) x := by
       rw[hcx, har]
-      simp only [padZeroes, List.length_replicate]
+      simp only [padZeros, List.length_replicate]
       rw[← List.append_assoc]
       simp only [List.length_replicate, List.append_replicate_replicate,
         List.append_cancel_right_eq, List.replicate_inj, AddLeftCancelMonoid.add_eq_zero,
@@ -178,7 +198,7 @@ theorem DFAO.bounded_out [Fintype state] (dfao : DFAO (Fin n → Fin (b+2)) stat
 
     by_cases hkb : k - b'.length ≤ Fintype.card state
     . have : Fintype.card state = (Fintype.card state - (k - b'.length)) + (k - b'.length) := by omega
-      rw[this, ← padZeroes_add (Fintype.card state - (k - b'.length)) (k - b'.length) x, ← hac]
+      rw[this, ← padZeros_add (Fintype.card state - (k - b'.length)) (k - b'.length) x, ← hac]
       apply h (a ++ c)
       . exact haco
     . simp only [not_le] at hkb
@@ -192,7 +212,7 @@ theorem DFAO.bounded_out [Fintype state] (dfao : DFAO (Fin n → Fin (b+2)) stat
       . exact hkb
       . rfl
 
-theorem DFA.bounded_accept [Fintype state] (dfa : DFA (Fin n → Fin (b+2)) state) (x : List (Fin n → Fin (b+2)))(h: dfa.acceptZero): ∀ z, (∃ k, z = padZeroes k x) ∧ dfa.eval z → dfa.eval (padZeroes (Fintype.card state) x) := by
+theorem DFA.bounded_accept [Fintype state] (dfa : DFA (Fin n → Fin (b+2)) state) (x : List (Fin n → Fin (b+2)))(h: dfa.acceptZero): ∀ z, (∃ k, z = padZeros k x) ∧ dfa.eval z → dfa.eval (padZeros (Fintype.card state) x) := by
   have := DFAO.bounded_out dfa x true
   intro z a
   simp_all only [implies_true, true_implies, DFA.acceptZero]
@@ -202,7 +222,7 @@ theorem DFA.bounded_accept [Fintype state] (dfa : DFA (Fin n → Fin (b+2)) stat
   apply this
   · exact right
 
-theorem NFA.bounded_accept [Fintype state] [DecidableEq state] (nfa : NFA (Fin n → Fin (b+2)) state) (x : List (Fin n → Fin (b+2)))(h: nfa.acceptZero): ∀ z, (∃ k, z = padZeroes k x) ∧ nfa.eval z → nfa.eval (padZeroes (Fintype.card (ListND state)) x) := by
+theorem NFA.bounded_accept [Fintype state] [DecidableEq state] (nfa : NFA (Fin n → Fin (b+2)) state) (x : List (Fin n → Fin (b+2)))(h: nfa.acceptZero): ∀ z, (∃ k, z = padZeros k x) ∧ nfa.eval z → nfa.eval (padZeros (Fintype.card (ListND state)) x) := by
   simp only [NFA.acceptZero, ← NFA.toDFA_eval] at *
   have := DFA.bounded_accept (nfa.toDFA) x h
   intro z a
@@ -216,17 +236,49 @@ theorem NFA.bounded_accept [Fintype state] [DecidableEq state] (nfa : NFA (Fin n
 
 def NFA.fixLeadingZeros [Fintype state] [DecidableEq state] (nfa : NFA (Fin n → Fin (b+2)) state) : NFA (Fin n → Fin (b+2)) state := {
   transition := nfa.transition
-  start := nfa.transFrom (padZeroes (Fintype.card (ListND state)) []) nfa.start
+  start := nfa.transFrom (padZeros (Fintype.card (ListND state)) []) nfa.start
   output := nfa.output
 }
 
+theorem NFA.fixLeadingZeros_transFrom [Fintype state] [DecidableEq state] (nfa : NFA (Fin n → Fin (b+2)) state) (s : List (Fin n → Fin (b+2))): (nfa.fixLeadingZeros).transFrom s nfa.fixLeadingZeros.start = nfa.transFrom (padZeros (Fintype.card (ListND state)) s) nfa.start := by
+  induction s using List.list_reverse_induction
+  case base =>
+    simp only [NFA.transFrom, NFA.fixLeadingZeros, padZeros]
+  case ind as a ih =>
+    simp[NFA.transFrom_of_append, ih]
+    nth_rw 2 [padZeros]
+    rw[← List.append_assoc]
+    rw[NFA.transFrom_of_append, padZeros]
+    rfl
+
+
+theorem NFA.fixLeadingZeros_eval [Fintype state] [DecidableEq state] (nfa : NFA (Fin n → Fin (b+2)) state) (x : List (Fin n → Fin (b+2))) : (nfa.fixLeadingZeros).eval x = nfa.eval (padZeros (Fintype.card (ListND state)) x) := by
+  simp only [NFA.eval, NFA.evalFrom]
+  rw[NFA.fixLeadingZeros_transFrom]
+  rfl
+
+theorem NFA.fixLeadingZeros.accept [Fintype state] [DecidableEq state] (nfa : NFA (Fin n → Fin (b+2)) state) (x : List (Fin n → Fin (b+2)))(h: nfa.acceptZero): ∀ z, (∃ k, z = padZeros k x) ∧ nfa.eval z → nfa.fixLeadingZeros.eval x := by
+  intro z a
+  simp only [NFA.fixLeadingZeros_eval]
+  apply NFA.bounded_accept
+  . exact h
+  . exact a
+
+theorem NFA.fixLeadingZeroes.acceptZero [Fintype state] [DecidableEq state] (nfa : NFA (Fin n → Fin (b+2)) state) (h: nfa.acceptZero): (nfa.fixLeadingZeros).acceptZero := by
+  simp_all only [NFA.acceptZero]
+  intro x h' m
+  rw[NFA.fixLeadingZeros_eval] at h'
+  rw[NFA.fixLeadingZeros_eval, padZeros_add]
+  simp only [add_comm]
+  rw[← padZeros_add]
+  simp_all only
 
 -- Legacy
 
 -- theorem equality_acceptZero : (eqBase (b + 2) l m n).acceptZero := by
 --   rw[DFA.acceptZero]
 --   intro x h c
---   rw[padZeroes]
+--   rw[padZeros]
 --   rw[DFAO.eval, DFAO.evalFrom, DFAO.transFrom_of_append]
 --   nth_rw 1 [eqBase]
 --   simp only [Fin.isValue, beq_iff_eq]
