Automata/Demos.lean
@@ -1,0 +1,23 @@
+import Mathlib.Tactic
+import Automata.Equality
+import Automata.Addition
+import Automata.Projection
+
+theorem zero_is_zero : 0 = 0 := by
+  apply (eqBase_iff_equal 2 (by norm_num) [0, 0] 2 (by norm_num) 0 1).mpr
+  rfl
+
+theorem foo : 100000 = 100000 := by
+  apply (eqBase_iff_equal 2 (by norm_num) [100000, 100000] 2 (by norm_num) 0 1).mpr
+  native_decide
+
+
+-- What's difficult
+-- ∃ x, x = 0?
+#eval (project 0 (eqBase 2 2 0 1)).eval [fun _ => 0]
+
+-- ∃ x, 1 + 1 = x?
+#eval (project 2 (addBase 2)).eval [fun _ => 1]
+-- Wrong! Why? Projection only searches for representations in restricted length, 1+1 = 2 needs 2 bits.
+#eval (project 2 (addBase 2)).eval [fun _ => 0, fun _ => 1]
+-- Correct after padding with 0s
